m2/m4 cast reimplemented

src/lib/data/Kuiper.Array4.fsti
@@ -14,6 +14,11 @@ module Tac = FStar.Tactics.V2
 let desc (d0 d1 d2 d3 : nat) : idesc 4 =
   d0 @| d1 @| d2 @| d3 @| INil
 
+// Even if this is trivial, it seems to help in some contexts.
+let sizeof_desc (d0 d1 d2 d3 : nat) : Lemma (sizeof (desc d0 d1 d2 d3) == d0 * d1 * d2 * d3)
+          [SMTPat (sizeof (desc d0 d1 d2 d3))]
+  = ()
+
 let ait (d0 d1 d2 d3 : nat) = natlt d0 & natlt d1 & natlt d2 & natlt d3
 
 let adapt_idx (#d0 #d1 #d2 #d3 : nat) (idx : abs (desc d0 d1 d2 d3)) : ait d0 d1 d2 d3 =
@@ -31,6 +36,36 @@ let cit_fits (d0 d1 d2 d3 : nat) (idx : raw_cit) : prop =
 
 [@@erasable]
 type layout (d0 d1 d2 d3 : nat) = tlayout (desc d0 d1 d2 d3)
+
+type full_layout (d0 d1 d2 d3 : nat) = l : layout d0 d1 d2 d3 { is_full l }
+
+let from_seq (#et:Type) (#d0 #d1 #d2 #d3 : nat)
+  (l : full_layout d0 d1 d2 d3)
+  (s : lseq et (d0 * d1 * d2 * d3))
+  : EMatrix4.t et d0 d1 d2 d3
+  = EMatrix4.mkM (fun i j k m -> s `Seq.index` l.imap.f (i, (j, (k, (m, ())))))
+
+let to_seq (#et:Type) (#d0 #d1 #d2 #d3 : nat)
+  (l : full_layout d0 d1 d2 d3)
+  (s : EMatrix4.t et d0 d1 d2 d3)
+  : GTot (lseq et (d0 * d1 * d2 * d3))
+  = Seq.init_ghost (d0 * d1 * d2 * d3) (fun i ->
+      let x = Kuiper.Injection.inverse_f l.imap i in
+      macc s x._1 x._2._1 x._2._2._1 x._2._2._2._1)
+
+// Odd that this seems to help.
+let to_seq_helper (#et:Type) (#d0 #d1 #d2 #d3 : nat)
+  (l : full_layout d0 d1 d2 d3)
+  (s : EMatrix4.t et d0 d1 d2 d3)
+  (i : natlt (d0 * d1 * d2 * d3))
+  : Lemma (to_seq l s `Seq.index` i == (let x = Kuiper.Injection.inverse_f l.imap i in macc s x._1 x._2._1 x._2._2._1 x._2._2._2._1))
+          [SMTPat (to_seq l s `Seq.index` i)]
+  = ()
+
+val to_from (#et:Type) (#d0 #d1 #d2 #d3 : nat)
+  (l : full_layout d0 d1 d2 d3) (s : lseq et (d0 * d1 * d2 * d3))
+  : Lemma (ensures to_seq l (from_seq l s) == s)
+          [SMTPat (to_seq l (from_seq l s))]
 
 let layout_size (#d0 #d1 #d2 #d3 : nat) (l : layout d0 d1 d2 d3) : GTot nat = l.ulen
 
@@ -105,6 +140,46 @@ fn pts_to_ref
     a |-> Frac f s
   ensures
     pure (SZ.fits (layout_size l))
+
+ghost
+fn concr
+  (#et:Type)
+  (#d0 #d1 #d2 #d3 : nat)
+  (#l : layout d0 d1 d2 d3 { is_full l })
+  (g : t et l)
+  (#s : EMatrix4.t et d0 d1 d2 d3)
+  (#f : perm)
+  requires
+    g |-> Frac f s
+  ensures
+    core g |-> Frac f (to_seq l s)
+
+ghost
+fn abs
+  (#et:Type)
+  (#d0 #d1 #d2 #d3 : nat)
+  (l : layout d0 d1 d2 d3 { is_full l })
+  (p : gpu_array et (layout_size l))
+  (#f : perm)
+  (#s : EMatrix4.t et d0 d1 d2 d3)
+  requires
+    p |-> Frac f (to_seq l s)
+  ensures
+    from_array l p |-> Frac f s
+
+ghost
+fn abs'
+  (#et:Type)
+  (#d0 #d1 #d2 #d3 : nat)
+  (l : layout d0 d1 d2 d3 { is_full l })
+  (p : gpu_array et (layout_size l))
+  (#f : perm)
+  (#s : lseq et (layout_size l))
+  requires
+    p |-> Frac f s
+  ensures
+    from_array l p |-> Frac f (from_seq l s)
+
 
 ghost
 fn share_n
