src/lib/data/Kuiper.Matrix.Casts.fst
@@ -6,50 +6,111 @@ open Kuiper
 // This should be restored to show how to cast a matrix into a tiled view via
 // concr/abs. But there is also a better API.
 
-(*
 module EM = Kuiper.EMatrix
-module M  = Kuiper.Matrix
-module M4 = Kuiper.Matrix4
+module A2 = Kuiper.Array2
+module A4 = Kuiper.Array4
+open Kuiper.EMatrix
+open Kuiper.EMatrix4
+
+let l2_to_l4 (#m #n : nat) (#mm #nn : pos) (l : A2.layout (m * mm) (n * nn)) : A4.layout m n mm nn = {
+  ulen = l.ulen;
+  imap =
+    Kuiper.Injection.mk_injection
+      (fun (i, (j, (k, (o, ())))) ->
+        let i : natlt m = i in
+        let j : natlt n = j in
+        let k : natlt mm = k in
+        let o : natlt nn = o in
+        let i : natlt (m * mm) = i * mm + k in
+        let j : natlt (n * nn) = j * nn + o in
+        l.imap.f (i, (j, ())))
+      (fun (i1, (j1, (k1, (o1, ()))))
+           (i2, (j2, (k2, (o2, ())))) ->
+           ())
+}
+
+let em2_to_em4 (#et : Type0) (#m #n #mm #nn : nat) (e : ematrix et (m * mm) (n * nn)) : ematrix4 et m n mm nn =
+  Kuiper.EMatrix4.mkM (fun i j k o -> Kuiper.EMatrix.macc e (i * mm + k) (j * nn + o))
+
+let l4_to_l2 (#m #n : nat) (#mm #nn : pos) (l : A4.layout m n mm nn) : A2.layout (m * mm) (n * nn) = {
+  ulen = l.ulen;
+  imap =
+    Kuiper.Injection.mk_injection #(natlt (m * mm) & (natlt (n * nn) & unit))
+      (fun (i, (j, ())) ->
+        let i : natlt m = i / mm in
+        let j : natlt n = j / nn in
+        let k : natlt mm = i % mm in
+        let o : natlt nn = j % nn in
+        l.imap.f (i, (j, (k, (o, ())))))
+      (fun (i1, (j1, ()))
+           (i2, (j2, ())) ->
+           admit())
+}
+
+let em4_to_em2 (#et : Type0) (#m #n #mm #nn : nat) (e : ematrix4 et m n mm nn) : ematrix et (m * mm) (n * nn) =
+  Kuiper.EMatrix.mkM (fun i j ->
+    let i : natlt m = i / mm in
+    let j : natlt n = j / nn in
+    let k : natlt mm = i % mm in
+    let o : natlt nn = j % nn in
+    Kuiper.EMatrix4.macc e i j k o)
 
 inline_for_extraction noextract
 fn m2_to_m4
-  (trows tcols mrows mcols : erased nat)
+  (m n mm nn : erased nat{mm > 0 /\ nn > 0})
   (#et : Type0) {| scalar et |}
-  (#lA : M4.mlayout4 mrows mcols trows tcols)
-  (gA : M.gpu_matrix et lA)
-  (#eA : EM.ematrix et _ _)
+  (#lA : A2.full_layout (m * mm) (n * nn))
+  (gA : A2.t et lA)
+  (#eA : ematrix et _ _)
   (#f : perm)
   requires
     gA |-> Frac f eA
   returns
-    gA4 : M4.gpu_matrix et lA
+    gA4 : A4.t et (l2_to_l4 lA)
   ensures
-    gA4 |-> Frac f eA **
-    pure (M4.core gA4 == M.core gA)
+    gA4 |-> Frac f (em2_to_em4 eA) **
+    pure (A4.core gA4 == A2.core gA)
 {
-  (* NICE ! *)
-  M.gpu_matrix_concr gA;
-  M4.gpu_matrix_abs lA (M.core gA);
-  M4.from_array lA (M.core gA);
+  (* Very roundabout way to do this. *)
+  A2.concr gA;
+  A4.abs' (l2_to_l4 lA) (A2.core gA);
+  let r = A4.from_array (l2_to_l4 lA) (A2.core gA);
+  assert rewrites_to r (A4.from_array (l2_to_l4 lA) (A2.core gA));
+  assert pure (Kuiper.EMatrix4.equal
+    (A4.from_seq (l2_to_l4 lA) (A2.to_seq lA eA))
+    (em2_to_em4 eA));
+  rewrite r |-> Frac f (A4.from_seq (l2_to_l4 lA) (A2.to_seq lA eA))
+       as r |-> Frac f (em2_to_em4 eA);
+  ();
+  r
 }
 
 inline_for_extraction noextract
 fn m4_to_m2
-  (#trows #tcols #mrows #mcols : erased nat)
+  (m n mm nn : erased nat{mm > 0 /\ nn > 0})
   (#et : Type0) {| scalar et |}
-  (#lA : M4.mlayout4 mrows mcols trows tcols)
-  (gA4 : M4.gpu_matrix et lA)
-  (#eA : EM.ematrix et _ _)
+  (#lA4 : A4.full_layout m n mm nn)
+  (gA4 : A4.t et lA4)
+  (#eA4 : ematrix4 et _ _ _ _)
   (#f : perm)
   requires
-    gA4 |-> Frac f eA
+    gA4 |-> Frac f eA4
   returns
-    gA : M.gpu_matrix et lA
+    gA : A2.t et (l4_to_l2 lA4)
   ensures
-    gA |-> Frac f eA **
-    pure (M4.core gA4 == M.core gA)
+    gA |-> Frac f (em4_to_em2 eA4) **
+    pure (A4.core gA4 == A2.core gA)
 {
-  M4.gpu_matrix_concr gA4;
-  M.gpu_matrix_abs lA (M4.core gA4);
-  M.from_array lA (M4.core gA4);
+  (* Very roundabout way to do this. *)
+  A4.concr gA4;
+  A2.abs' (l4_to_l2 lA4) (A4.core gA4);
+  let r = A2.from_array (l4_to_l2 lA4) (A4.core gA4);
+  assert rewrites_to r (A2.from_array (l4_to_l2 lA4) (A4.core gA4));
+  assert pure (Kuiper.EMatrix.equal
+    (A2.from_seq (l4_to_l2 lA4) (A4.to_seq lA4 eA4))
+    (em4_to_em2 eA4));
+  rewrite r |-> Frac f (A2.from_seq (l4_to_l2 lA4) (A4.to_seq lA4 eA4))
+       as r |-> Frac f (em4_to_em2 eA4);
+  ();
+  r
 }
