src/lib/ghost/Kuiper.Ghost.TensorTranspose.fst
@@ -20,14 +20,14 @@ fn ghost_transpose1
   ensures
     row2col gA |-> mtranspose m
 {
-  array2_concr gA;
+  concr gA;
   assume_ (pure (Seq.equal
                   (to_seq (l2_row_major rows cols) m)
                   (to_seq (l2_col_major cols rows) (mtranspose m))));
   // FIXME: ^ should be obvious
   rewrite core gA |-> to_seq (l2_row_major rows cols) m
        as core gA |-> to_seq (l2_col_major cols rows) (mtranspose m);
-  array2_abs (l2_col_major cols rows) (core gA);
+  abs (l2_col_major cols rows) (core gA);
 }
 
 ghost
@@ -41,14 +41,14 @@ fn ghost_transpose2
   ensures
     col2row gA |-> mtranspose m
 {
-  array2_concr gA;
+  concr gA;
   assume_ (pure (Seq.equal
                   (to_seq (l2_col_major rows cols) m)
                   (to_seq (l2_row_major cols rows) (mtranspose m))));
   // FIXME: ^ should be obvious
   rewrite core gA |-> to_seq (l2_col_major rows cols) m
        as core gA |-> to_seq (l2_row_major cols rows) (mtranspose m);
-  array2_abs (l2_row_major cols rows) (core gA);
+  abs (l2_row_major cols rows) (core gA);
 }
 
 ghost
